BlockCacheSystem/JournalDiskUtils.i.dfy
@@ -1,0 +1,214 @@
+include "DiskLayout.i.dfy"
+include "AsyncSectorDiskModel.i.dfy"
+
+module JournalDiskUtils {
+  import opened DiskLayout
+  import opened NativeTypes
+  import opened JournalRanges
+  import opened SectorType
+  import opened AsyncSectorDisk
+  import opened Journal
+  import opened Options
+
+  type DiskConstants = AsyncSectorDisk.Constants
+  type DiskState = AsyncSectorDisk.Variables
+
+  predicate WFRange(start: int, len: int)
+  {
+    && 0 <= start < NumJournalBlocks() as int
+    && 0 <= len <= NumJournalBlocks() as int
+  }
+
+  predicate Disk_HasJournalRange(
+      blocks: imap<Location, Sector>, start: int, len: int)
+  requires WFRange(start, len)
+  {
+    && (JournalFrontLocation(start as uint64, len as uint64).Some? ==>
+      && JournalFrontLocation(start as uint64, len as uint64).value in blocks
+      && blocks[JournalFrontLocation(start as uint64, len as uint64).value].SectorJournal?
+    )
+    && (JournalBackLocation(start as uint64, len as uint64).Some? ==>
+      && JournalBackLocation(start as uint64, len as uint64).value in blocks
+      && blocks[JournalBackLocation(start as uint64, len as uint64).value].SectorJournal?
+    )
+  }
+
+  function Disk_JournalRange(blocks: imap<Location, Sector>, start: int, len: int) : JournalRange
+  requires WFRange(start, len)
+  requires Disk_HasJournalRange(blocks, start, len)
+  {
+    if JournalBackLocation(start as uint64, len as uint64).Some? then
+      JournalRangeConcat(
+          blocks[JournalFrontLocation(start as uint64, len as uint64).value].journal,
+          blocks[JournalBackLocation(start as uint64, len as uint64).value].journal)
+    else if JournalFrontLocation(start as uint64, len as uint64).Some? then
+      blocks[JournalFrontLocation(start as uint64, len as uint64).value].journal
+    else
+      JournalRangeEmpty()
+  }
+
+  protected predicate Disk_HasJournal(
+      blocks: imap<Location, Sector>, start: int, len: int)
+  requires WFRange(start, len)
+  {
+    && Disk_HasJournalRange(blocks, start, len)
+    && parseJournalRange(Disk_JournalRange(blocks, start, len)).Some?
+  }
+
+  protected function Disk_Journal(
+      blocks: imap<Location, Sector>, start: int, len: int) : seq<JournalEntry>
+  requires WFRange(start, len)
+  requires Disk_HasJournal(blocks, start, len)
+  {
+    parseJournalRange(Disk_JournalRange(blocks, start, len)).value
+  }
+
+  predicate NoOverlaps(reqWrites: map<ReqId, ReqWrite>)
+  {
+    forall id1, id2 | id1 in reqWrites && id2 in reqWrites ::
+        !overlap(reqWrites[id1.loc], reqWrites[id2.loc])
+  }
+
+  function Disk_JournalBlockAtLoc(blocks: imap<Location, Sector>, loc: Location)
+    : Option<JournalRange>
+  {
+    if loc in blocks && blocks[loc].SectorJournal? then
+      Some(blocks[loc].journal)
+    else
+      None
+  }
+
+  function Disk_JournalBlockAt(blocks: imap<Location, Sector>, i: int)
+    : Option<JournalRange>
+  requires 0 <= i < NumJournalBlocks()
+  {
+    Disk_JournalBlockAtLoc(blocks, JournalRangeLocation(i, 1))
+  }
+
+  function Queue_JournalBlockAt(reqWrites: map<ReqId, ReqWrite>, i: int)
+    : Option<JournalRange>
+  requires 0 <= i < NumJournalBlocks()
+  {
+    var loc := JournalRangeLocation(i, 1);
+    if id :| id in reqWrites && LocationSub(loc, reqWrites[id].loc) then (
+      if reqWrites[loc].sector.SectorJournal?
+         && 0 <= i - JournalBlockIdx(reqWrites[id].loc) < 
+            JournalRangeLen(reqWrites[loc].sector.journal) then (
+        Some(JournalBlockGet(reqWrites[loc].sector.journal,
+            i - JournalBlockIdx(reqWrites[id].loc)))
+      ) else (
+        None
+      )
+    ) else (
+      None
+    )
+  }
+
+  function DiskQueue_JournalBlockAt(disk: DiskState, i: int)
+    : Option<JournalRange>
+  requires 0 <= i < NumJournalBlocks()
+  {
+    if Queue_JournalBlockAt(disk.reqWrites, i).Some? then
+      Queue_JournalBlockAt(disk.reqWrites, i)
+    else
+      Disk_JournalBlockAt(disk.blocks, i)
+  }
+
+  function DiskQueue_JournalBlockSeq_i(disk: DiskState, i: int)
+    : (res : seq<Option<JournalRange>>)
+  requires 0 <= i <= NumJournalBlocks()
+  ensures |res| == i
+  ensures forall j | 0 <= j < i :: res[j] == DiskQueue_JournalBlockAt(disk, j)
+  {
+    if i == 0 then [] else
+      Disk_JournalBlockSeq_i(disk, i-1) + [DiskQueue_JournalBlockAt(disk, i-1)]
+  }
+
+  function DiskQueue_JournalBlockSeq(disk: DiskState)
+  ensures forall j | 0 <= j < NumJournalBlocks() :: res[j] == DiskQueue_JournalBlockAt(disk, j)
+  {
+    Disk_JournalBlockSeq_i(disk, NumJournalBlocks())
+  }
+
+  predicate DiskQueue_HasJournalRange(
+      disk: DiskState, start: int, len: int)
+  requires WFRange(start, len)
+  {
+    NoOverlapsInRange(disk.reqWrites, 
+  }
+
+  function DiskQueue_JournalRange(
+      disk: DiskState, start: int, len: int) : JournalRange
+  requires WFRange(start, len)
+  requires DiskQueue_HasJournal(disk, start, len)
+
+
+
+
+  protected predicate DiskQueue_HasJournal(
+      disk: DiskState, start: int, len: int)
+  requires WFRange(start, len)
+
+  protected function DiskQueue_Journal(
+      disk: DiskState, start: int, len: int) : seq<JournalEntry>
+  requires WFRange(start, len)
+  requires DiskQueue_HasJournal(disk, start, len)
+
+  lemma Disk_eq_DiskQueue(disk: DiskState, start: int, len: int)
+  requires WFRange(start, len)
+  requires Disk_HasJournal(disk.blocks, start, len)
+  requires forall id | id in disk.reqWrites ::
+      locDisjointFromCircularJournalRange(
+          disk.reqWrites[id].loc, start as uint64, len as uint64)
+  ensures DiskQueue_HasJournal(disk, start, len)
+  ensures Disk_Journal(disk.blocks, start, len)
+      == DiskQueue_Journal(disk, start, len)
+
+  lemma Disk_Journal_empty(disk: DiskState, start: int)
+  requires WFRange(start, 0)
+  ensures Disk_HasJournal(disk.blocks, start, 0)
+  ensures Disk_Journal(disk.blocks, start, 0) == []
+
+  lemma DiskQueue_Journal_empty(disk: DiskState, start: int)
+  requires WFRange(start, 0)
+  ensures DiskQueue_HasJournal(disk, start, 0)
+  ensures DiskQueue_Journal(disk, start, 0) == []
+
+  lemma DiskQueue_Journal_append(
+      k: DiskConstants, disk: DiskState, disk': DiskState,
+      start: int, len: int, jr: JournalRange,
+      dop: DiskOp)
+  requires WFRange(start, len)
+  requires AsyncSectorDisk.RecvWrite(k, disk, disk', dop)
+  requires DiskQueue_HasJournal(disk, start, len)
+  requires parseJournalRange(jr).Some?
+  requires len + JournalRangeLen(jr) <= NumJournalBlocks() as int
+  requires JournalPosAdd(start, len) + JournalRangeLen(jr) <= NumJournalBlocks() as int
+  ensures DiskQueue_HasJournal(disk', start, len + JournalRangeLen(jr))
+  ensures DiskQueue_Journal(disk', start, len + JournalRangeLen(jr))
+      == DiskQueue_Journal(disk, start, len) + parseJournalRange(jr).value
+
+  lemma DiskQueue_Journal_ProcessWrite(
+      k: DiskConstants, disk: DiskState, disk': DiskState,
+      start: int, len: int,
+      id: ReqId)
+  requires WFRange(start, len)
+  requires AsyncSectorDisk.ProcessWrite(k, disk, disk', id)
+  requires DiskQueue_HasJournal(disk, start, len)
+  ensures DiskQueue_HasJournal(disk', start, len)
+  ensures DiskQueue_Journal(disk', start, len)
+       == DiskQueue_Journal(disk, start, len)
+
+  lemma Disk_Journal_ProcessWrite(
+      k: DiskConstants, disk: DiskState, disk': DiskState,
+      start: int, len: int,
+      id: ReqId)
+  requires WFRange(start, len)
+  requires AsyncSectorDisk.ProcessWrite(k, disk, disk', id)
+  requires Disk_HasJournal(disk.blocks, start, len)
+  requires locDisjointFromCircularJournalRange(
+          disk.reqWrites[id].loc, start as uint64, len as uint64)
+  ensures Disk_HasJournal(disk'.blocks, start, len)
+  ensures Disk_Journal(disk'.blocks, start, len)
+       == Disk_Journal(disk.blocks, start, len)
+}
